CTree/LTS.lean
@@ -7,37 +7,39 @@ namespace CTree
 
   inductive Label (ε : Type → Type) (ρ : Type)
   | val (v : ρ)
-  | event (α : Type) (e : ε α) (a : α)
+  | event (α : Type) (e : ε α)
+  | response (α : Type) (e : ε α) (a : α)
   | tau
 
-  inductive Step : CTree ε ρ → Label ε ρ → CTree ε ρ → Prop
-  | ret : Step (ret v) (.val v) zero
-  | vis {α} {e : ε α} {a : α} {k : α → CTree ε ρ} : Step (vis e k) (.event α e a) (k a)
-  | tau : Step t.tau .tau t
-  | choice_left (h : Step t1 l t3) : Step (t1 ⊕ t2) l t3
-  | choice_right (h : Step t2 l t3) : Step (t1 ⊕ t2) l t3
+  inductive Step : State ε ρ → Label ε ρ → State ε ρ → Prop
+  | ret : Step (C[ ret v ]) (.val v) (C[ zero ])
+  | event {α} {e : ε α} {k : α → CTree ε ρ} : Step (C[ vis e k ]) (.event α e) (K[ k ])
+  | response {α} {e : ε α} {a : α} {k : α → CTree ε ρ} : Step (K[ k ]) (.response α e a) (C[ k a ])
+  | tau : Step (C[ t.tau ]) .tau (C[ t ])
+  | choice_left (h : Step (C[ t1 ]) l t3) : Step (C[ t1 ⊕ t2 ]) l t3
+  | choice_right (h : Step (C[ t2 ]) l t3) : Step (C[ t1 ⊕ t2 ]) l t3
 
-  def NTauStep (n : Nat) (t1 t3 : CTree ε ρ) : Prop :=
+  def NTauStep (n : Nat) (t1 t3 : State ε ρ) : Prop :=
     match n with
     | 0 => t1 = t3
     | n + 1 => ∃ t2, Step t1 .tau t2 ∧ NTauStep n t2 t3
 
-  def WeakStep (t1 : CTree ε ρ) (l : Label ε ρ) (t4 : CTree ε ρ) : Prop :=
+  def WeakStep (t1 : State ε ρ) (l : Label ε ρ) (t4 : State ε ρ) : Prop :=
     ∃ t2 t3 n1 n2, NTauStep n1 t1 t2 ∧ Step t2 l t3 ∧ NTauStep n2 t3 t4
 
-  def IsWeakSimulation (sim : Rel (CTree ε ρ) (CTree ε ρ)) : Prop :=
+  def IsWeakSimulation (sim : Rel (State ε ρ) (State ε ρ)) : Prop :=
     ∀ p1 q1, sim p1 q1 →
       ∀ l p2, Step p1 l p2 →
         match l with
         | .tau => ∃ n q2, NTauStep n q1 q2 ∧ sim p2 q2
         | _ => ∃ q2, WeakStep q1 l q2 ∧ sim p2 q2
 
-  def IsWeakBisimulation (sim : Rel (CTree ε ρ) (CTree ε ρ)) : Prop :=
+  def IsWeakBisimulation (sim : Rel (State ε ρ) (State ε ρ)) : Prop :=
     IsWeakSimulation sim ∧ IsWeakSimulation (flip sim)
 
-  def WeakSim : Rel (CTree ε ρ) (CTree ε ρ) :=
+  def WeakSim : Rel (State ε ρ) (State ε ρ) :=
     λ p q => ∃ sim, IsWeakSimulation sim ∧ sim p q
 
-  def WeakBisim : Rel (CTree ε ρ) (CTree ε ρ) :=
+  def WeakBisim : Rel (State ε ρ) (State ε ρ) :=
     λ p q => ∃ sim, IsWeakBisimulation sim ∧ sim p q
 end CTree
